src/Proofs/TransferFrom.v
@@ -51,11 +51,18 @@ Definition _now_right (rec: Type) (def: XDefault rec) := \\ now \\.
 
 Opaque Common.hmapFindWithDefault
         CommonInstances.addAdjustListPair
-        N.add N.sub N.leb N.ltb N.eqb Z.eqb.
+        N.add N.sub N.leb N.ltb N.eqb Z.eqb N.pow.
 
 Axiom EqSome: forall (a b: XUBInteger 256),
 a = b -> Some a = Some b.
 
+
+Lemma if_transit: forall X Y (b: bool) (f: X -> Y) x y, 
+  f (if b then x else y) = if b then f x else f y.
+Proof.
+  intros.
+  destruct b; auto.
+Qed.
 
 Lemma transferFrom_set_from_balance: forall
                             (_from :  address)
@@ -76,90 +83,54 @@ Lemma transferFrom_set_from_balance: forall
 Proof.        
     intros. subst l'.
     rewrite <- transferFrom_prf.
+
     destruct l. repeat destruct p.   
     destruct v. repeat destruct p.
     destruct c. repeat destruct p.  
 
-    compute.
+    unfold transferFrom_exec.    
+    repeat rewrite exec_if_transit, exec_if_transit2.
 
-    match goal with
-    | |- context [@addAdjustListPair _ _ _ _to ?v _] => remember v
-    end.
+    (*repeat rewrite if_transit. *)
+
+
+    compute.
+    compute in _from_balance0, allowance0, msg_sender.  
+
+    assert (forall n (v1 v: XUBInteger n) (T11 T12: _ -> Type) T2 f w w1, 
+    ((let 'Build_XUBInteger a as a'' := v
+    return T11 a'' -> T2 in
+    fun _: T11 a'' => (let 'Build_XUBInteger b as b'' := v1
+    return T12 b''-> T2 in fun _ : T12 b'' => f b a) w) w1) = 
+    f (uint2N v1) (uint2N v)).
+
+    intros.
+
+    destruct v, v1. auto.
+    rewrite ?H0.
 
     match goal with
     | |- context [if ?b then false else true] => remember b
     end.    
 
-     case_eq b; intros; auto.
-     erewrite lookup_some_find.
-    reflexivity.
-    unshelve erewrite lookup_addAdjust.
-    refine (BoolEq.pair_eqb_spec (X:=Z) (Y:=XUBInteger 256)).
-
-
-    apply EqSome.
-    erewrite lookup_some_find.
-    reflexivity.
-
-    unshelve erewrite lookup_addAdjust_another.
-    refine (BoolEq.pair_eqb_spec (X:=Z) (Y:=XUBInteger 256)).
-(*     erewrite find_lookup.
-    reflexivity.
-
-
-
- reflexivity.
-
-    auto.
-    assumption. *)
-
-Qed.
-
-(* Lemma transfer_set_recepient_balance: forall (_to :  address) 
-                            (_value : uint256)
-                            (l: LedgerLRecord rec), 
-    let l0 := {$$ l with Ledger_LocalState := default $$} in
-    let l' := exec_state (Uinterpreter (@transfer rec def _ _ _ _ _to _value)) l0 in
-    let msg_sender := VMState_ι_msg_sender (l.(Ledger_VMState)) in
-    let msg_sender_balance0 := (_balances (l.(Ledger_MainState))) [msg_sender] in
-    let recepient_balance0 := (_balances (l.(Ledger_MainState))) [_to] in
-    _to <> msg_sender -> 
-    (_balances (l'.(Ledger_MainState))) [_to] = 
-        if (xIntGeb msg_sender_balance0  _value : bool) then 
-        xIntPlus recepient_balance0 _value
-        else recepient_balance0.
-Proof.        
-    intros. subst l'.
-    rewrite <- transfer_prf.
-    destruct l. repeat destruct p.   
-    destruct v. repeat destruct p.
-    destruct c. repeat destruct p.
-
-    compute.
-
-    match goal with
-    | |- context [@addAdjustListPair ?K ?V ?H a ?v ?m] => remember (@addAdjustListPair K V H a v m)
-    end.
-
-    match goal with
-    | |- context [if ?b then false else true] => remember b
-    end.    
-    
     case_eq b; intros; auto.
 
-    erewrite lookup_some_find.
-    reflexivity.    
 
+    match goal with
+    | |- context [if ?b then _ else _] => remember b
+    end.
+
+    case_eq b0; intros.
+
+    -    
+    erewrite lookup_some_find.
+    reflexivity.
     unshelve erewrite lookup_addAdjust.
     refine (BoolEq.pair_eqb_spec (X:=Z) (Y:=XUBInteger 256)).
 
-    subst l3.
-
-    remember (x10 [_to] ?).
+    remember (x10 [_from] ?).
     destruct y.
-
-    - 
-    erewrite lookup_some_find.
+    + erewrite lookup_some_find.
     reflexivity. 
     unshelve erewrite lookup_addAdjust_another.
     refine (BoolEq.pair_eqb_spec (X:=Z) (Y:=XUBInteger 256)).
@@ -170,14 +141,221 @@ Proof.
     reflexivity.
     assumption. 
 
-    -
-    rewrite lookup_none_find.
-    rewrite lookup_none_find.
-    reflexivity.
-    setoid_rewrite Heqy. reflexivity.
+    + rewrite lookup_none_find.
+    * rewrite lookup_none_find.
+      reflexivity.
+      setoid_rewrite Heqy. 
+      reflexivity.
 
+    * unshelve erewrite lookup_addAdjust_another.
+      refine (BoolEq.pair_eqb_spec (X:=Z) (Y:=XUBInteger 256)).
+      setoid_rewrite <- Heqy. reflexivity. 
+      assumption.
+
+    -  erewrite lookup_some_find.
+    reflexivity.
+    unshelve erewrite lookup_addAdjust.
+    refine (BoolEq.pair_eqb_spec (X:=Z) (Y:=XUBInteger 256)).
+
+    remember (x10 [_from] ?).
+    destruct y.
+    + erewrite lookup_some_find.
+    reflexivity. 
     unshelve erewrite lookup_addAdjust_another.
     refine (BoolEq.pair_eqb_spec (X:=Z) (Y:=XUBInteger 256)).
-    setoid_rewrite <- Heqy. reflexivity. 
+    erewrite lookup_some_find.
+    setoid_rewrite <- Heqy.    
+    reflexivity. 
+    setoid_rewrite <- Heqy.
+    reflexivity.
+    assumption. 
+
+    + rewrite lookup_none_find.
+    * rewrite lookup_none_find.
+      reflexivity.
+      setoid_rewrite Heqy. 
+      reflexivity.
+
+    * unshelve erewrite lookup_addAdjust_another.
+      refine (BoolEq.pair_eqb_spec (X:=Z) (Y:=XUBInteger 256)).
+      setoid_rewrite <- Heqy. reflexivity. 
+      assumption.
+Qed.
+
+
+Lemma transferFrom_set_to_balance: forall
+                            (_from :  address)
+                            (_to :  address)
+                            (_value : uint256)
+                            (l: LedgerLRecord rec), 
+    let l0 := {$$ l with Ledger_LocalState := default $$} in
+    let l' := exec_state (Uinterpreter (@transferFrom rec def _ _ _ _ _from _to _value)) l0 in
+    let msg_sender := VMState_ι_msg_sender (l.(Ledger_VMState)) in
+    let _from_balance0 := (_balances (l.(Ledger_MainState))) [_from] in
+    let _to_balance0 := (_balances (l.(Ledger_MainState))) [_to] in
+    let allowance := (_allowed(l.(Ledger_MainState)))[_from][msg_sender] in
+    _to <> _from -> 
+(*     (xIntGeb allowance  _value : bool) = true ->
+ *)    (_balances (l'.(Ledger_MainState))) [_to] = 
+        if ((xIntGeb _from_balance0  _value : bool)  && (xIntGeb allowance  _value : bool) ) then 
+                xIntPlus _to_balance0 _value
+        else _to_balance0.
+Proof.        
+    intros. subst l'.
+    rewrite <- transferFrom_prf.
+
+    destruct l. repeat destruct p.   
+    destruct v. repeat destruct p.
+    destruct c. repeat destruct p.  
+
+    unfold transferFrom_exec.    
+    repeat rewrite exec_if_transit, exec_if_transit2.
+
+    (*repeat rewrite if_transit. *)
+
+
+    compute.
+    compute in _from_balance0, _to_balance0, allowance0, msg_sender.  
+
+    assert (forall n (v1 v: XUBInteger n) (T11 T12: _ -> Type) T2 f w w1, 
+    ((let 'Build_XUBInteger a as a'' := v
+    return T11 a'' -> T2 in
+    fun _: T11 a'' => (let 'Build_XUBInteger b as b'' := v1
+    return T12 b''-> T2 in fun _ : T12 b'' => f b a) w) w1) = 
+    f (uint2N v1) (uint2N v)).
+
+    intros.
+
+    destruct v, v1. auto.
+    rewrite ?H0.
+
+    match goal with
+    | |- context [if ?b then false else true] => remember b
+    end.    
+
+    case_eq b; intros; auto.
+
+
+    match goal with
+    | |- context [if ?b then _ else _] => remember b
+    end.
+
+    case_eq b0; intros.
+
+    -          
+    erewrite lookup_some_find.
+    reflexivity.
+    unshelve erewrite lookup_addAdjust_another.
+    refine (BoolEq.pair_eqb_spec (X:=Z) (Y:=XUBInteger 256)).
+    unshelve erewrite lookup_addAdjust.
+    refine (BoolEq.pair_eqb_spec (X:=Z) (Y:=XUBInteger 256)).
+
+    auto.
     assumption.
-Qed. *)
+
+    -
+
+    erewrite lookup_some_find.
+    reflexivity.
+    unshelve erewrite lookup_addAdjust_another.
+    refine (BoolEq.pair_eqb_spec (X:=Z) (Y:=XUBInteger 256)).
+    unshelve erewrite lookup_addAdjust.
+    refine (BoolEq.pair_eqb_spec (X:=Z) (Y:=XUBInteger 256)).
+
+    auto.
+    assumption.
+Qed.
+
+Check toValue (eval_state (sRReader (MAX_UINT256_right rec def)) _).
+
+Print intFunRec_gen.
+
+
+Lemma transferFrom_set_allowed: forall
+                            (_from :  address)
+                            (_to :  address)
+                            (_value : uint256)
+                            (l: LedgerLRecord rec), 
+    let l0 := {$$ l with Ledger_LocalState := default $$} in
+    let l' := exec_state (Uinterpreter (@transferFrom rec def _ _ _ _ _from _to _value)) l0 in
+    let msg_sender := VMState_ι_msg_sender (l.(Ledger_VMState)) in
+    let _from_balance0 := (_balances (l.(Ledger_MainState))) [_from] in    
+    let allowed0 := (_allowed(l.(Ledger_MainState)))[_from][msg_sender] in  
+    let MAX_UINT256 := toValue (eval_state (sRReader (MAX_UINT256_right rec def)) l0) in
+      (_allowed (l'.(Ledger_MainState))) [_from][msg_sender] = 
+        if ((xIntGeb _from_balance0  _value : bool)  && (xIntGeb allowed0  _value : bool) ) then 
+                if (xIntGtb MAX_UINT256 allowed0: bool) then xIntMinus allowed0 _value else allowed0
+        else allowed0.
+Proof.        
+    intros. subst l'.
+    rewrite <- transferFrom_prf.
+
+    destruct l. repeat destruct p.   
+    destruct v. repeat destruct p.
+    destruct c. repeat destruct p.  
+
+    unfold transferFrom_exec.    
+    repeat rewrite exec_if_transit, exec_if_transit2.
+
+    compute.
+    compute in _from_balance0, allowed0, msg_sender.  
+
+    assert (forall n (v1 v: XUBInteger n) (T11 T12: _ -> Type) T2 f w w1, 
+    ((let 'Build_XUBInteger a as a'' := v
+    return T11 a'' -> T2 in
+    fun _: T11 a'' => (let 'Build_XUBInteger b as b'' := v1
+    return T12 b''-> T2 in fun _ : T12 b'' => f b a) w) w1) = 
+    f (uint2N v1) (uint2N v)).
+
+    intros.
+
+    destruct v, v1. auto.
+    rewrite ?H.
+
+
+    assert (forall n (v: XUBInteger n) (T11: _ -> Type) T2 f w, 
+    (let 'Build_XUBInteger a as a'' := v
+    return T11 a'' -> T2 in
+    fun _: T11 a'' => f a) w = 
+    f (uint2N v)).
+
+    intros.
+
+    destruct v. auto.
+    rewrite ?H0.
+
+
+    assert (forall X n (v: XUBInteger n) (f : _ -> X), 
+     match v with 
+      | Build_XUBInteger x => f x
+      end = f (uint2N v) ).
+
+    intros.
+
+    destruct v. auto.
+    rewrite ?H1.
+
+    match goal with
+    | |- context [if ?b then false else true] => remember b
+    end.    
+
+    case_eq b; intros; auto.
+
+    match goal with
+    | |- context [if ?b then _ else _] => remember b
+    end.
+
+    case_eq b0; intros; auto.
+
+    erewrite lookup_some_find with (k:=_from).
+    2: unshelve erewrite lookup_addAdjust.
+    2: refine (BoolEq.pair_eqb_spec (X:=Z) (Y:=XUBInteger 256)).
+    2: reflexivity.
+
+    erewrite lookup_some_find with (k:=a).
+    reflexivity.
+
+    unshelve erewrite lookup_addAdjust.
+    refine (BoolEq.pair_eqb_spec (X:=Z) (Y:=XUBInteger 256)).
+    reflexivity.
+Qed.
